Update timing proofs to use new generalizations

timing/examples/FreeRTOS/list/uxListRemove.v
@@ -1,30 +1,34 @@
-Require Import RTOSDemo_NoAsserts_Clz.
-Require Import riscvTiming.
+Require Import RTOSDemo.
+Require Import RISCVTiming.
 Import RISCVNotations.
-Require Import timing_auto.
 
-(* Common for all timing proofs - facilitates automation *)
-Module uxListRemoveTime <: TimingModule.
-    Definition time_of_addr (s : store) (a : addr) : N :=
-        match neorv32_cycles_upper_bound s (RTOSDemo_NoAsserts_Clz a) with
-        | Some x => x | _ => 999 end.
+Module TimingProof (cpu : CPUTimingBehavior).
 
+Module Program_uxListRemove <: ProgramInformation.
     Definition entry_addr : N := 0x80002440.
 
     Definition exits (t:trace) : bool :=
-    match t with (Addr a,_)::_ => match a with
-    | 0x80002470 => true
-    | _ => false
-  end | _ => false end.
-End uxListRemoveTime.
-Module uxListRemoveAuto := TimingAutomation uxListRemoveTime.
-Import uxListRemoveTime uxListRemoveAuto.
+        match t with (Addr a,_)::_ => match a with
+        | 0x80002470 => true
+        | _ => false
+    end | _ => false end.
+
+    Definition binary := RTOSDemo.
+End Program_uxListRemove.
+
+Module RISCVTiming := RISCVTiming cpu Program_uxListRemove.
+Module uxListRemoveAuto := RISCVTimingAutomation RISCVTiming.
+Import Program_uxListRemove uxListRemoveAuto.
 
 (* Postcondition *)
-Definition time_of_uxListRemove (t : trace) (base_mem : addr -> N) (a0 : N) :=
-    cycle_count_of_trace t = 6 * time_mem +
-        (if base_mem Ⓓ[4 + base_mem Ⓓ[16 + a0]] =? a0 then 3 + time_mem else time_branch) + 
-        3 * time_mem + 2 + time_branch.
+Definition time_of_uxListRemove (t : trace) (mem : addr -> N) (a0 : N) :=
+    cycle_count_of_trace t =
+        tlw + tlw + tlw + tsw + tsw + tlw +
+        (if mem Ⓓ[4 + mem Ⓓ[16 + a0]] =? a0 then
+            tfbne + tsw 
+         else
+            ttbne) +
+        tsw + tlw + taddi + tsw + tjalr.
 
 (* These values are used frequently, so we give them names for readability *)
 (* https://github.com/FreeRTOS/FreeRTOS-Kernel/blob/main/include/list.h#L143 *)
@@ -60,15 +64,14 @@ match t with (Addr a, s) :: t' => match a with
                         cycle_count_of_trace t' = 0)
 | 0x80002460 => Some (exists mem, s V_MEM32 = Ⓜmem /\
                         noverlaps mem a0 /\
-                        cycle_count_of_trace t' = 6 * time_mem +
-                            (if base_mem Ⓓ[4 + base_mem Ⓓ[16 + a0]] =? a0 then 3 + time_mem else time_branch))
-| 0x80002470 => Some (exists mem, s V_MEM32 = Ⓜmem /\ 
-                        time_of_uxListRemove t base_mem a0)
+                        cycle_count_of_trace t' = 
+                            tlw + tlw + tlw + tsw + tsw + tlw +
+                            (if base_mem Ⓓ[4 + base_mem Ⓓ[16 + a0]] =? a0 then 
+                                tfbne + tsw 
+                            else
+                                ttbne))
+| 0x80002470 => Some (time_of_uxListRemove t base_mem a0)
 | _ => None end | _ => None end.
-
-(* Lift the program *)
-Definition lifted_uxListRemove : program :=
-    lift_riscv RTOSDemo_NoAsserts_Clz.
 
 Theorem uxListRemove_timing:
   forall s t s' x' base_mem a0
@@ -78,7 +81,7 @@ Theorem uxListRemove_timing:
          (MEM: s V_MEM32 = Ⓜbase_mem)
          (A0: s R_A0 = Ⓓa0),
   satisfies_all 
-    lifted_uxListRemove
+    lifted_prog
     (uxListRemove_timing_invs base_mem a0)
     exits
   ((x',s')::t).
@@ -86,8 +89,8 @@ Proof using.
     (* Specialize some automation tactics for our purposes *)
     Local Ltac step := time rv_step.
     Local Ltac unfold_noverlap :=
-        unfold pxNext, pxPrevious, pxContainer, pxIndex, 
-            noverlaps, memory_regions in *.
+        unfold noverlaps, memory_regions,
+            pxNext, pxPrevious, pxContainer, pxIndex in *.
     Local Ltac preserve_noverlaps := 
         noverlaps_preserved unfold_noverlap.
 
@@ -122,14 +125,14 @@ Proof using.
             preserve_noverlaps.
         hammer.
         unfold_noverlap. unfold_create_noverlaps.
-        rewrite getmem_noverlap, getmem_noverlap in BC by 
+        rewrite getmem_noverlap, getmem_noverlap in BC by
             (auto using noverlap_symmetry).
         find_rewrites. lia.
     }
 
     (* Postcondition - `repeat step` got us here (repeat is weird) *)
     destruct PRE as (mem & MEM & NVL & Cycles).
-    repeat step. eexists. split. reflexivity.
-    unfold time_of_uxListRemove. hammer.
+    repeat step. unfold time_of_uxListRemove. hammer.
 Qed.
 
+End TimingProof.
