timing/examples/FreeRTOS/tasks/prvResetNextTaskUnblockTime.v
@@ -1,32 +1,33 @@
-Require Import RTOSDemo_NoAsserts_Clz.
-Require Import riscvTiming.
+Require Import RTOSDemo.
+Require Import RISCVTiming.
 Import RISCVNotations.
-Require Import timing_auto.
 
-Module prvResetNextTaskUnblockTimeTime <: TimingModule.
-    Definition time_of_addr (s : store) (a : addr) : N :=
-        match neorv32_cycles_upper_bound s (RTOSDemo_NoAsserts_Clz a) with
-        | Some x => x | _ => 999 end.
+Module TimingProof (cpu : CPUTimingBehavior).
 
+Module Program_prvResetNextTaskUnblockTime <: ProgramInformation.
     Definition entry_addr : N := 0x80000478.
 
     Definition exits (t:trace) : bool :=
-    match t with (Addr a,_)::_ => match a with
-    | 0x8000048c => true
-    | _ => false
-  end | _ => false end.
-End prvResetNextTaskUnblockTimeTime.
+        match t with (Addr a,_)::_ => match a with
+        | 0x8000048c => true
+        | _ => false
+    end | _ => false end.
 
-Module prvResetNextTaskUnblockTimeAuto := TimingAutomation prvResetNextTaskUnblockTimeTime.
-Import prvResetNextTaskUnblockTimeTime prvResetNextTaskUnblockTimeAuto.
+    Definition binary := RTOSDemo.
+End Program_prvResetNextTaskUnblockTime.
+
+Module RISCVTiming := RISCVTiming cpu Program_prvResetNextTaskUnblockTime.
+Module prvResetNextTaskUnblockTimeAuto := RISCVTimingAutomation RISCVTiming.
+Import Program_prvResetNextTaskUnblockTime prvResetNextTaskUnblockTimeAuto.
 
 Definition time_of_prvResetNextTaskUnblockTime (mem : addr -> N) (gp : N) (t : trace) :=
-    cycle_count_of_trace t = 2 * time_mem +
-        (if mem Ⓓ[mem Ⓓ[(0 ⊖ 1900) + gp]] =? 0 then 
-            3 + 2
+    cycle_count_of_trace t =
+        tlw + tlw +
+        (if mem Ⓓ[mem Ⓓ[gp ⊖ 1900]] =? 0 then 
+            tfbne + taddi
          else
-            time_branch + 3 * time_mem + time_branch) +
-        time_mem + time_branch.
+            ttbne + tlw + tlw + tlw + tjal) +
+        tsw + tjalr.
 
 Definition prvResetNextTaskUnblockTime_timing_invs (s : store) (base_mem : addr -> N) (gp : N)
     (t:trace) : option Prop :=
@@ -35,13 +36,6 @@ match t with (Addr a, s) :: t' => match a with
 | 0x8000048c => Some (time_of_prvResetNextTaskUnblockTime base_mem gp t)
 | _ => None end | _ => None end.
 
-Definition lifted_prvResetNextTaskUnblockTime : program :=
-    lift_riscv RTOSDemo_NoAsserts_Clz.
-
-(* We use simpl in a few convenient places: make sure it doesn't go haywire *)
-Arguments N.add _ _ : simpl nomatch.
-Arguments N.mul _ _ : simpl nomatch.
-
 Theorem prvResetNextTaskUnblockTime_timing:
   forall s t s' x' base_mem gp
          (ENTRY: startof t (x',s') = (Addr entry_addr, s))
@@ -49,7 +43,7 @@ Theorem prvResetNextTaskUnblockTime_timing:
          (MEM: s V_MEM32 = Ⓜbase_mem)
          (GP: s R_GP = Ⓓgp),
   satisfies_all 
-    lifted_prvResetNextTaskUnblockTime
+    lifted_prog
     (prvResetNextTaskUnblockTime_timing_invs s base_mem gp)
     exits
   ((x',s')::t).
@@ -69,10 +63,11 @@ Proof using.
     destruct_inv 32 PRE.
 
     destruct PRE as (MEM & GP & Cycles).
-    repeat step.
+    repeat step; fold_big_subs.
     unfold time_of_prvResetNextTaskUnblockTime.
         hammer.
     unfold time_of_prvResetNextTaskUnblockTime.
         hammer.
 Qed.
 
+End TimingProof.
