timing/examples/FreeRTOS/tasks/vTaskSuspendAll.v
@@ -1,7 +1,8 @@
-Require Import RTOSDemo_NoAsserts_Clz.
+Require Import RTOSDemo.
 Require Import RISCVTiming.
-Require Import NEORV32.
 Import RISCVNotations.
+
+Module TimingProof (cpu : CPUTimingBehavior).
 
 Module Program_vTaskSuspendAll <: ProgramInformation.
     Definition entry_addr : N := 0x80000d14.
@@ -12,10 +13,10 @@ Module Program_vTaskSuspendAll <: ProgramInformation.
         | _ => false
     end | _ => false end.
 
-    Definition binary := RTOSDemo_NoAsserts_Clz.
+    Definition binary := RTOSDemo.
 End Program_vTaskSuspendAll.
 
-Module RISCVTiming := RISCVTiming NEORV32Base Program_vTaskSuspendAll.
+Module RISCVTiming := RISCVTiming cpu Program_vTaskSuspendAll.
 Module vTaskSuspendAllAuto := RISCVTimingAutomation RISCVTiming.
 Import Program_vTaskSuspendAll vTaskSuspendAllAuto.
 
@@ -30,27 +31,12 @@ match t with (Addr a, s) :: t' => match a with
 | 0x80000d20 => Some (time_of_vTaskSuspendAll t)
 | _ => None end | _ => None end.
 
-Definition lifted_vTaskSuspendAll : program :=
-    lift_riscv RTOSDemo_NoAsserts_Clz.
-
-(* We use simpl in a few convenient places: make sure it doesn't go haywire *)
-Arguments N.add _ _ : simpl nomatch.
-Arguments N.mul _ _ : simpl nomatch.
-
-Lemma fold_left_add_base_0 : forall l base,
-    List.fold_left N.add l base = base + List.fold_left N.add l 0.
-Proof.
-    induction l; intros; simpl.
-        lia.
-    now rewrite IHl, <- N.add_assoc, <- (IHl a).
-Qed. 
-
 Theorem vTaskSuspendAll_timing:
   forall s t s' x'
          (ENTRY: startof t (x',s') = (Addr entry_addr, s))
          (MDL: models rvtypctx s),
   satisfies_all 
-    lifted_vTaskSuspendAll
+    lifted_prog
     (vTaskSuspendAll_timing_invs)
     exits
   ((x',s')::t).
@@ -73,3 +59,4 @@ Proof using.
     hammer.
 Qed.
 
+End TimingProof.
